rocq-skylabs-cpp2v/tests/location_unsupported_perf.t/large_check.v
@@ -1,3 +1,4 @@
+Require Import Stdlib.Numbers.Cyclic.Int63.Uint63.
 Require Import skylabs.lang.cpp.syntax.source_location.
 Require Import skylabs.lang.cpp.parser.
 Require Import large_17_cpp_locations.
@@ -10,7 +11,7 @@ Definition last_root : decl_root :=
       (core.Nfunction function_qualifiers.N "large_15"
         [Tnum int_rank.Iint Signed])).
 
-Definition first_line (result : lookup_error + list source_origin) : option N :=
+Definition first_line (result : lookup_error + list source_origin) : option PrimInt63.int :=
   match result with
   | inr (origin :: _) =>
       match origin.(spelling_range) with
@@ -27,5 +28,5 @@ Definition first_line (result : lookup_error + list source_origin) : option N :=
 Example large_tu_deep_lookup_reduces :
     first_line
       (skylabs.lang.cpp.syntax.source_location.lookup source_locations
-        last_root [0; 2; 0; 0; 0; 1]) = Some 17%N.
+        last_root [0; 2; 0; 0; 0; 1]) = Some 17%uint63.
 Proof. vm_compute. reflexivity. Qed.
